Deterministic step relation

theories/Map.v
@@ -54,7 +54,7 @@ Arguments for_all {T} p m : rename, simpl never.
 Lemma for_all_spec {T P p} (R : forall k (v : T), Reflect.Bool (P k v) (p k v)) m
   : Reflect.Bool (ForAll P m) (for_all p m).
 Proof.
-  cbn in *. unfold ForAll. unfold Find. rewrite MapCore.for_all_spec. eapply (Reflect.bool_eq (forall k v
+  cbn in *. unfold ForAll. unfold Find. rewrite MapCore.for_all_spec. eapply (@Reflect.bool_eq (forall k v
     (F : SetoidList.InA MapCore.eq_key_elt (k, v) (MapCore.bindings m)), P k v)). {
     split; intros H k v; [rewrite MapCore.bindings_spec1 | rewrite <- MapCore.bindings_spec1]; apply H. }
   remember (MapCore.bindings m) as bindings eqn:Eb; clear m Eb.
@@ -141,6 +141,11 @@ Qed.
 Lemma in_eq {T} {m1 m2 : to T} (E : Eq m1 m2) x
   : In m1 x <-> In m2 x.
 Proof. split; intros [y F]; eexists; apply E; exact F. Qed.
+
+
+
+Definition InRange {T} (m : to T) v := exists k, Find m k v.
+Arguments InRange {T} m v/.
 
 
 
@@ -343,30 +348,68 @@ Lemma add_det
 Proof. cbn in *. intros x y. subst. rewrite A1. rewrite A2. rewrite Em. reflexivity. Qed.
 
 Lemma add_eq
-  k1 {T} (v1 : T) m1 m' (A1 : Add k1 v1 m1 m')
+  k1 {T} (v1 : T) m1 m1' (A1 : Add k1 v1 m1 m1')
   k2 (Ek : k1 = k2)
   v2 (Ev : v1 = v2)
   m2 (Em : Eq m1 m2)
-  : Add k2 v2 m2 m'.
+  m2' (Em' : Eq m1' m2')
+  : Add k2 v2 m2 m2'.
 Proof.
   subst. split.
-  - intro F. apply A1 in F as [[-> ->] | F]; [left | right]. { split; reflexivity. } apply Em. exact F.
-  - intro F. apply A1. destruct F as [[-> ->] | F]; [left | right]. { split; reflexivity. } apply Em. exact F.
+  - intro F. apply Em' in F. apply A1 in F as [[-> ->] | F]; [left | right]. { split; reflexivity. } apply Em. exact F.
+  - intro F. apply Em'. apply A1. destruct F as [[-> ->] | F]; [left | right]. { split; reflexivity. } apply Em. exact F.
+Qed.
+
+
+
+Definition OverwriteIfPresent {T} k v (m m' : to T) : Prop :=
+  forall x y, (Find m' x y <-> ((x = k /\ y = v) \/ (x <> k /\ Find m x y))).
+Arguments OverwriteIfPresent {T} k v m m'/.
+
+Definition overwrite := @overriding_add.
+Arguments overwrite {T} k v m/.
+
+Lemma overwrite_if_present_overwrite {T} k m (v : T)
+  : OverwriteIfPresent k v m (overwrite k v m).
+Proof. cbn. intros. apply find_overriding_add. Qed.
+
+Lemma overwrite_if_present_det {T}
+  k1 (v1 : T) m1 m1' (O1 : OverwriteIfPresent k1 v1 m1 m1')
+  k2 (Ek : k1 = k2)
+  v2 (Ev : v1 = v2)
+  m2 (Em : Eq m1 m2)
+  m2' (O2 : OverwriteIfPresent k2 v2 m2 m2')
+  : Eq m1' m2'.
+Proof. cbn in *. intros x y. subst. rewrite O1. rewrite O2. cbn in Em. rewrite Em. reflexivity. Qed.
+
+Lemma overwrite_if_present_eq {T}
+  k1 (v1 : T) m1 m1' (O1 : OverwriteIfPresent k1 v1 m1 m1')
+  k2 (Ek : k1 = k2)
+  v2 (Ev : v1 = v2)
+  m2 (Em : Eq m1 m2)
+  m2' (Em' : Eq m1' m2')
+  : OverwriteIfPresent k2 v1 m2 m2'.
+Proof. cbn in *. subst. intros. cbn in Em'. rewrite <- Em'. rewrite O1. cbn in Em. rewrite Em. reflexivity. Qed.
+
+Lemma in_overwrite_if_present {T k v m m'} (O : @OverwriteIfPresent T k v m m') x
+  : In m' x <-> (x = k \/ In m x).
+Proof.
+  split.
+  - intros [y F]. apply O in F as [[-> ->] | [N F]]; [left | right]. { reflexivity. } eexists. exact F.
+  - intros [-> | [y F]]. { eexists. apply O. left. split; reflexivity. }
+    destruct (Name.spec x k); subst; eexists; apply O; [left | right]. { split; reflexivity. } split; eassumption.
 Qed.
 
 
 
 Definition Overwrite {T} k v (m m' : to T) : Prop :=
   In m k /\ (* <-- this proof should be easy wherever `Overwrite` is used, but it's a sanity check *)
-  forall x y, (Find m' x y <-> ((x = k /\ y = v) \/ (x <> k /\ Find m x y))).
+  OverwriteIfPresent k v m m'.
 Arguments Overwrite {T} k v m m'/.
-
-Definition overwrite := @overriding_add.
-Arguments overwrite {T} k v m/.
 
 Lemma overwrite_overwrite {T} k m (I : In m k) (v : T)
   : Overwrite k v m (overwrite k v m).
-Proof. split. { exact I. } intros. apply find_overriding_add. Qed.
+Proof. split. { exact I. } apply overwrite_if_present_overwrite. Qed.
 
 Lemma overwrite_det {T}
   k1 (v1 : T) m1 m1' (O1 : Overwrite k1 v1 m1 m1')
@@ -375,20 +418,18 @@ Lemma overwrite_det {T}
   m2 (Em : Eq m1 m2)
   m2' (O2 : Overwrite k2 v2 m2 m2')
   : Eq m1' m2'.
-Proof.
-  intros x y. subst. destruct O1 as [I1 O1]. destruct O2 as [I2 O2].
-  rewrite O1. rewrite O2. cbn in Em. rewrite Em. reflexivity.
-Qed.
+Proof. destruct O1 as [I1 O1]. destruct O2 as [I2 O2]. eapply overwrite_if_present_det; eassumption. Qed.
 
 Lemma overwrite_eq {T}
-  k1 (v1 : T) m1 m' (O1 : Overwrite k1 v1 m1 m')
+  k1 (v1 : T) m1 m1' (O : Overwrite k1 v1 m1 m1')
   k2 (Ek : k1 = k2)
   v2 (Ev : v1 = v2)
   m2 (Em : Eq m1 m2)
-  : Overwrite k2 v1 m2 m'.
+  m2' (Em' : Eq m1' m2')
+  : Overwrite k2 v1 m2 m2'.
 Proof.
-  subst. destruct O1 as [I1 O1]. split. { eapply in_eq. { apply eq_sym. exact Em. } exact I1. }
-  intros. rewrite O1. cbn in Em. rewrite Em. reflexivity.
+  subst. destruct O as [I O]. split. 2: { eapply overwrite_if_present_eq; try reflexivity; eassumption. }
+  eapply in_eq. { apply eq_sym. exact Em. } exact I.
 Qed.
 
 Lemma in_overwrite {T k v m m'} (O : @Overwrite T k v m m') x
@@ -399,6 +440,68 @@ Proof.
   destruct (Name.spec x k). { eexists. apply O. left. split. { exact Y. } reflexivity. }
   eexists. apply O. right. split. { exact N. } exact F.
 Qed.
+
+
+
+Definition RemoveIfPresent {T} k (m m' : to T) : Prop :=
+  forall x y, (Find m' x y <-> (x <> k /\ Find m x y)).
+Arguments RemoveIfPresent {T} k m m'/.
+
+Definition remove := @MapCore.remove.
+Arguments remove {T} k m : rename, simpl never.
+
+Lemma remove_if_present_remove {T} k (m : to T)
+  : RemoveIfPresent k m (remove k m).
+Proof.
+  cbn. intros. rewrite find_iff. unfold find. unfold remove. destruct (Name.spec k x).
+  - subst. rewrite MapCore.remove_spec1. split. { intro D. discriminate D. } intros [C _]. contradiction C. reflexivity.
+  - rewrite MapCore.remove_spec2. 2: { exact N. } fold (find m x). rewrite <- find_iff.
+    split. { intro F. split. { symmetry. exact N. } exact F. } intros [_ F]. exact F.
+Qed.
+
+Lemma remove_if_present_det {T k1} {m1 m1' : to T} (R1 : RemoveIfPresent k1 m1 m1')
+  {k2} (Ek : k1 = k2)
+  {m2} (Em : Map.Eq m1 m2)
+  {m2'} (R2 : RemoveIfPresent k2 m2 m2')
+  : Map.Eq m1' m2'.
+Proof. subst. cbn in *. intros x y. rewrite R1. rewrite R2. cbn in Em. rewrite Em. reflexivity. Qed.
+
+Lemma in_remove_if_present {T k} {m m' : to T} (R : RemoveIfPresent k m m') x
+  : In m' x <-> (x <> k /\ In m x).
+Proof.
+  split.
+  - intros [y F]. apply R in F as [N F]. split. { exact N. } eexists. exact F.
+  - intros [N [y F]]. eexists. apply R. split. { exact N. } exact F.
+Qed.
+
+Lemma find_remove_if_present {T k} {m m' : to T} (R : RemoveIfPresent k m m') x y
+  : Find m' x y <-> (x <> k /\ Find m x y).
+Proof.
+  split.
+  - intro F. apply R in F as [N F]. split. { exact N. } exact F.
+  - intros [N F]. apply R. split. { exact N. } exact F.
+Qed.
+
+
+
+Definition Remove {T} k (m m' : to T) : Prop :=
+  In m k /\ RemoveIfPresent k m m'.
+Arguments Remove {T} k m m'/.
+
+Lemma remove_remove {T k} {m : to T} (I : In m k)
+  : Remove k m (remove k m).
+Proof. split. { exact I. } apply remove_if_present_remove. Qed.
+
+Lemma remove_det {T k1} {m1 m1' : to T} (R1 : Remove k1 m1 m1')
+  {k2} (Ek : k1 = k2)
+  {m2} (Em : Map.Eq m1 m2)
+  {m2'} (R2 : Remove k2 m2 m2')
+  : Map.Eq m1' m2'.
+Proof. eapply remove_if_present_det. { apply R1. } { exact Ek. } { exact Em. } apply R2. Qed.
+
+Lemma in_remove {T k} {m m' : to T} (R : Remove k m m') x
+  : In m' x <-> (x <> k /\ In m x).
+Proof. apply in_remove_if_present. apply R. Qed.
 
 
 
@@ -413,7 +516,7 @@ Arguments agree {T} eqb a/ b.
 Lemma agree_spec {T eqb} (eqb_spec : forall a b : T, Reflect.Bool (a = b) (eqb a b)) a b
   : Reflect.Bool (Agree a b) (agree eqb a b).
 Proof.
-  apply (Reflect.bool_eq (Agree b a)). { cbn. split; intros; specialize (H _ _ F0 _ F) as ->; reflexivity. }
+  apply (@Reflect.bool_eq (Agree b a)). { cbn. split; intros; specialize (H _ _ F0 _ F) as ->; reflexivity. }
   apply for_all_spec. intros. apply agree_on_spec. exact eqb_spec.
 Qed.
 
@@ -470,7 +573,7 @@ Proof.
       * destruct (find_spec a x). { apply N in Y as []. } apply find_iff. exact F.
 Qed.
 
-Lemma union_overriding_union {T} {a b : to T} (A : Agree a b)
+Lemma union_overriding {T} {a b : to T} (A : Agree a b)
   : Union a b (overriding_union a b).
 Proof.
   split.
@@ -486,10 +589,10 @@ Lemma find_checked_union {T eqb} {a b c : to T} (E : checked_union eqb a b = Som
   : find c x = match find a x with Some y => Some y | None => find b x end.
 Proof. unfold checked_union in E. destruct agree in E; invert E. apply find_overriding_union. Qed.
 
-Lemma union_checked_union {T eqb} (eqb_spec : forall a b : T, Reflect.Bool (a = b) (eqb a b))
+Lemma union_checked {T eqb} (eqb_spec : forall a b : T, Reflect.Bool (a = b) (eqb a b))
   {a b c} (E : checked_union eqb a b = Some c)
   : Union a b c.
-Proof. unfold checked_union in E. destruct (agree_spec eqb_spec a b); invert E. apply union_overriding_union. exact Y. Qed.
+Proof. unfold checked_union in E. destruct (agree_spec eqb_spec a b); invert E. apply union_overriding. exact Y. Qed.
 
 Lemma union_iff {T eqb} (eqb_spec : forall a b : T, Reflect.Bool (a = b) (eqb a b)) (a b c : to T)
   : Union a b c <-> exists c', (checked_union eqb a b = Some c' /\ Eq c c').
@@ -498,11 +601,238 @@ Proof.
     split. 2: { intros [? [D _]]. discriminate D. } intro U. contradiction N. eapply union_agree. eassumption. }
   eassert (Iff : (exists c', _) <-> forall k v, (Find c k v <-> Find (overriding_union a b) k v)); [| rewrite Iff]. {
     split. { intros [? [tmp E]]; invert tmp. exact E. } intro E. eexists. split. { reflexivity. } exact E. }
-  split; intros U' k v; rewrite U'; [symmetry |]; apply union_overriding_union; exact Y.
+  split; intros U' k v; rewrite U'; [symmetry |]; apply union_overriding; exact Y.
 Qed.
+
+Lemma union_det {T}
+  {a1 b1 c1} (U1 : @Union T a1 b1 c1)
+  {a2} (Ea : Eq a1 a2)
+  {b2} (Eb : Eq b1 b2)
+  {c2} (U2 : Union a2 b2 c2)
+  : Eq c1 c2.
+Proof. cbn in *. intros x y. rewrite U1. rewrite U2. rewrite Ea. rewrite Eb. reflexivity. Qed.
 
 
 
 Definition Reflect (P : Name.name -> Prop) (p : set) : Prop :=
   forall x, (In p x <-> P x).
 Arguments Reflect P p/.
+
+
+
+(*
+Definition Map {X Y} (f : Name.name -> X -> Y) m m' : Prop :=
+  forall k, (
+    (forall v (F : Find m k v), Find m' k (f k v)) /\
+    (forall (N : ~In m k) (I : In m' k), False)
+  ).
+Arguments Map {X Y} f m m'/.
+*)
+
+Definition map : forall X Y, (Name.name -> X -> Y) -> Map.to X -> Map.to Y := @MapCore.mapi.
+Arguments map {X Y} f m : simpl never.
+
+
+
+Definition domain {T} : to T -> set := map (fun k v => tt).
+Arguments domain {T} m/.
+
+Lemma find_domain {T} k v (m : to T)
+  : Find (domain m) k v <-> In m k.
+Proof.
+  destruct v. assert (Iff : In m k <-> exists v, SetoidList.InA MapCore.eq_key_elt (k, v) (MapCore.bindings m)). {
+    split; intros [v' F]; exists v'; apply MapCore.bindings_spec1; exact F. }
+  rewrite Iff; clear Iff. unfold Find. rewrite <- MapCore.bindings_spec1. unfold domain. unfold map.
+  rewrite MapCore.mapi_spec. remember (MapCore.bindings m) as b eqn:Eb; clear m Eb; rename b into m.
+  generalize dependent k. induction m as [| [x y] tail IH]; intros; cbn in *. {
+    split; [intro I | intros [v' I]]; invert I. } split; [intro I | intros [v' I]].
+  - invert I. { destruct H0; cbn in *; subst. eexists. left. split; reflexivity. }
+    apply IH in H0 as [v' I]. eexists. right. exact I.
+  - invert I. { destruct H0; cbn in *; subst. left. split; reflexivity. }
+    right. apply IH. eexists. exact H0.
+Qed.
+
+
+
+Definition fold {X Y} (f : Name.name -> X -> Y -> Y) (acc : Y) (m : to X) : Y := @MapCore.fold X Y f m acc.
+Arguments fold {X Y} f acc m : simpl never.
+
+
+
+Definition Minus {T} (everything : to T) (discard : set) (subtracted : to T) : Prop :=
+  forall k v, Find subtracted k v <-> (Find everything k v /\ forall (discarded : In discard k), False).
+Arguments Minus {T} everything discard subtracted/.
+
+Definition minus {T} : to T -> set -> to T := fold (fun k _ acc => remove k acc).
+Arguments minus {T} everything discard/.
+
+Lemma minus_minus {T} (everything : to T) discard
+  : Minus everything discard (minus everything discard).
+Proof.
+  cbn. intros. unfold fold. rewrite MapCore.fold_spec. assert (Iff :
+    (Find everything k v /\ (forall (discarded : exists v, Find discard k v), False)) <->
+    (Find everything k v /\ (forall (discarded : exists v,
+      SetoidList.InA MapCore.eq_key_elt (k, v) (MapCore.bindings discard)), False))). {
+    split; intros [F N]; (split; [exact F |]); intros [v' N'];
+    apply N; exists v'; apply MapCore.bindings_spec1; exact N'. } rewrite Iff; clear Iff.
+  remember (MapCore.bindings discard) as b eqn:Eb; clear discard Eb; rename b into discard.
+  generalize dependent k. generalize dependent T. induction discard as [| [k v] tail IH]; intros; cbn in *. {
+    split. { intro F. split. { exact F. } intros [v' I]. invert I. } intros [F N]. exact F. }
+  rewrite IH; clear IH. split; intros [F N].
+  - eapply find_remove_if_present in F as [Nk F]. 2: { apply remove_if_present_remove. }
+    split. { exact F. } intros [v' C]. apply N. invert C. 2: { eexists. eassumption. }
+    destruct H0; cbn in *; subst. contradiction Nk. reflexivity.
+  - split. 2: { intros [v' C]. apply N. eexists. right. exact C. }
+    eapply find_remove_if_present. { apply remove_if_present_remove. } split. 2: { exact F. }
+    intros ->. apply N. eexists. left. split; reflexivity.
+Qed.
+
+
+
+Definition BulkOverwrite {T} (force original overwritten : to T) : Prop :=
+  forall x y, (Find overwritten x y <-> (Find force x y \/ ((forall (I : In force x), False) /\ Find original x y))).
+Arguments BulkOverwrite {T} force original overwritten/.
+
+Definition bulk_overwrite := @overriding_union.
+Arguments bulk_overwrite {T} a b/.
+
+Lemma bulk_overwrite_bulk_overwrite {T} (force original : to T)
+  : BulkOverwrite force original (bulk_overwrite force original).
+Proof.
+  intros x y. rewrite find_iff. rewrite find_overriding_union. split.
+  - intro E. destruct (find_spec force x); [left | right]. { invert E. exact Y. }
+    split. 2: { apply find_iff. exact E. } intros [f F]. apply N in F as [].
+  - intros [F | [N F]]. { apply find_iff in F. rewrite F. reflexivity. }
+    destruct (find_spec force x). { edestruct N. eexists. exact Y. } apply find_iff. exact F.
+Qed.
+
+Lemma bulk_overwrite_det {T}
+  {f1 o1 y1 : to T} (O1 : BulkOverwrite f1 o1 y1)
+  {f2} (Ef : Eq f1 f2)
+  {o2} (Eo : Eq o1 o2)
+  {y2} (O2 : BulkOverwrite f2 o2 y2)
+  : Eq y1 y2.
+Proof.
+  cbn in *. intros. rewrite O1. rewrite O2. assert (A := in_eq Ef).
+  cbn in A. rewrite A. rewrite Ef. rewrite Eo. reflexivity.
+Qed.
+
+Lemma bulk_overwrite_eq {T}
+  {f1 o1 y1 : to T} (O1 : BulkOverwrite f1 o1 y1)
+  {f2} (Ef : Eq f1 f2)
+  {o2} (Eo : Eq o1 o2)
+  {y2} (Ey : Eq y1 y2)
+  : BulkOverwrite f2 o2 y2.
+Proof.
+  cbn in *. intros. rewrite <- Ey. rewrite O1. assert (A := in_eq Ef).
+  cbn in A. rewrite A. rewrite Ef. rewrite Eo. reflexivity.
+Qed.
+
+Lemma in_bulk_overwrite {T force original overwritten} (O : @BulkOverwrite T force original overwritten) x
+  : In overwritten x <-> (In force x \/ ((forall (I : In force x), False) /\ In original x)).
+Proof.
+  split.
+  - intros [y F]. apply O in F as [F | [N F]]; [left | right]. { eexists. exact F. }
+    split. { exact N. } eexists. exact F.
+  - intros [[y F] | [N [y F]]]; eexists; apply O; [left | right]. { exact F. } split. { exact N. } exact F.
+Qed.
+
+
+
+Definition ToSelf (domain : set) to_self : Prop :=
+  forall x y, Find to_self x y <-> (In domain x /\ x = y).
+Arguments ToSelf domain to_self/.
+
+Definition to_self : set -> to Name.name := map (fun k _ => k).
+Arguments to_self domain/.
+
+Lemma to_self_to_self domain
+  : ToSelf domain (to_self domain).
+Proof.
+  cbn in *. intros x y. unfold Find at 1. rewrite <- MapCore.bindings_spec1. unfold map. rewrite MapCore.mapi_spec.
+  fold (In domain x). assert (Iff : In domain x <-> exists y,
+    SetoidList.InA MapCore.eq_key_elt (x, y) (MapCore.bindings domain)). {
+    split; intros [y' F]; exists y'; apply MapCore.bindings_spec1; exact F. }
+  rewrite Iff; clear Iff. remember (MapCore.bindings domain) as b eqn:Eb; clear domain Eb. rename b into domain.
+  generalize dependent y. generalize dependent x. induction domain as [| [k v] tail IH]; intros; cbn in *. {
+    split. { intro I. invert I. } intros [[y' I] E]. invert I. } split.
+  - intro I. invert I. { destruct H0; cbn in *; subst. split. { eexists. left. split; reflexivity. } reflexivity. }
+    apply IH in H0 as [[y' I] ->]. split. 2: { reflexivity. } eexists. right. exact I.
+  - intros [[y' I] ->]. invert I. { destruct H0; cbn in *; subst. left. split; reflexivity. }
+    right. apply IH. split. 2: { reflexivity. } eexists. eassumption.
+Qed.
+
+Lemma in_to_self domain x
+  : In (to_self domain) x <-> In domain x.
+Proof.
+  split; intros [y F]. { apply to_self_to_self in F as [I ->]. exact I. }
+  eexists. apply to_self_to_self. split. { eexists. exact F. } reflexivity.
+Qed.
+
+Lemma to_self_det {d1 y1} (TS1 : ToSelf d1 y1)
+  {d2} (Ed : Map.Eq d1 d2)
+  {y2} (TS2 : ToSelf d2 y2)
+  : Eq y1 y2.
+Proof.
+  split; intro F; [apply TS1 in F | apply TS2 in F]; destruct F as [I E]; [apply TS2 | apply TS1];
+  (split; [| exact E]); (eapply in_eq; [| exact I]); try assumption; apply eq_sym; assumption.
+Qed.
+
+
+
+Lemma sorted_lt {T}
+  {kv : _ * T} {tail} (S : Sorted.Sorted MapCore.lt_key tail) (L : Sorted.HdRel MapCore.lt_key kv tail)
+  (N : ~SetoidList.InA MapCore.eq_key kv tail) (ND : SetoidList.NoDupA MapCore.eq_key tail)
+  {xy} (I : SetoidList.InA MapCore.eq_key_elt xy tail)
+  : MapCore.lt_key kv xy.
+Proof.
+  generalize dependent xy. generalize dependent ND. generalize dependent kv.
+  induction S; intros; invert I; destruct xy as [x y]; destruct kv as [k v]; destruct a as [k' v'].
+  - destruct H1; cbn in *; subst. invert L. assumption.
+  - invert L. invert ND.  apply IHS; try assumption. 2: { intro I. apply N. right. exact I. }
+    destruct l. { invert H1. } constructor. eapply Name.trans. { eassumption. } invert H. assumption.
+Qed.
+
+Lemma bindings_eq {T} a b
+  : @Eq T a b <-> MapCore.bindings a = MapCore.bindings b.
+Proof.
+  split; intro E.
+  - assert (Sa := MapCore.bindings_spec2 a). assert (Sb := MapCore.bindings_spec2 b).
+    assert (NDa := MapCore.bindings_spec2w a). assert (NDb := MapCore.bindings_spec2w b).
+    assert (Iff : Eq a b <-> forall x y, (
+      SetoidList.InA MapCore.eq_key_elt (x, y) (MapCore.bindings a) <->
+      SetoidList.InA MapCore.eq_key_elt (x, y) (MapCore.bindings b))). {
+      split; intros E' x y; specialize (E' x y); [repeat rewrite MapCore.bindings_spec1 |
+        repeat rewrite MapCore.bindings_spec1 in E']; exact E'. }
+    rewrite Iff in E; clear Iff.
+    remember (MapCore.bindings a) as ba eqn:Ea; clear a Ea; rename ba into a.
+    remember (MapCore.bindings b) as bb eqn:Eb; clear b Eb; rename bb into b.
+    generalize dependent b. generalize dependent NDa.
+    induction Sa as [| [ka va] a' Sa' IH La]; intros; cbn in *. {
+      destruct b as [| [k v] tail]. { reflexivity. } assert (A : SetoidList.InA MapCore.eq_key_elt
+        (k, v) ((k, v) :: tail)). { left. split; reflexivity. } apply E in A. invert A. }
+    invert NDa as [| ? ? Na NDa']. invert NDb as [| shit b' Nb NDb']. {
+      assert (A : SetoidList.InA MapCore.eq_key_elt (ka, va) ((ka, va) :: a')). { left. split; reflexivity. }
+      apply E in A. invert A. }
+    invert Sb as [| [kb vb] b Sb' Lb]. destruct (Name.compare_spec ka kb).
+    + cbn in H. subst. f_equal.
+      * f_equal. specialize (E kb vb).
+        assert (A : SetoidList.InA MapCore.eq_key_elt (kb, vb) ((kb, vb) :: b')). { left. split; reflexivity. }
+        apply E in A. invert A. { destruct H0; cbn in *; subst. reflexivity. }
+        contradiction Na. clear Sa' La IH b' E Nb NDb' Sb' Lb Na NDa'.
+        induction a'; invert H0; [left | right]. { apply H1. } apply IHa'. assumption.
+      * apply IH; try assumption. split; intro I; (eassert (I' : SetoidList.InA _ _ _); [right; exact I |]);
+        apply E in I'; (invert I'; [| assumption]); destruct H0; cbn in *; subst; [contradiction Na | contradiction Nb];
+        cbn; clear Sa' La IH Na E NDa' Nb NDb' Sb' Lb; (induction I; [left; apply H | right; exact IHI]).
+    + assert (A : SetoidList.InA MapCore.eq_key_elt (ka, va) ((kb, vb) :: b')). { apply E. left. split; reflexivity. }
+      invert A as [| ? ? I]. { destruct H0; cbn in *; subst. rewrite Name.compare_refl in H. discriminate H. }
+      assert (L : MapCore.lt_key (kb, vb) (ka, va)). { eapply sorted_lt; try exact I; eassumption. }
+      unfold MapCore.lt_key in L. cbn in L. unfold Name.lt in H.
+      rewrite Name.antisym in L. rewrite H in L. discriminate L.
+    + assert (A : SetoidList.InA MapCore.eq_key_elt (kb, vb) ((ka, va) :: a')). { apply E. left. split; reflexivity. }
+      invert A as [| ? ? I]. { destruct H0; cbn in *; subst. rewrite Name.compare_refl in H. discriminate H. }
+      assert (L : MapCore.lt_key (ka, va) (kb, vb)). { eapply sorted_lt; try exact I; eassumption. }
+      unfold MapCore.lt_key in L. cbn in L. unfold Name.lt in H.
+      rewrite Name.antisym in L. rewrite H in L. discriminate L.
+  - intros x y. unfold Find. repeat rewrite <- MapCore.bindings_spec1. rewrite E. reflexivity.
+Qed.
