theories/Match.v
@@ -4,6 +4,7 @@ From LinearCore Require
   Map
   Pattern
   Term
+  WellFormed
   .
 From LinearCore Require Import
   Invert
@@ -23,10 +24,10 @@ Inductive Strict (context : Context.context) : Pattern.strict -> Term.term -> Co
         : Map.Add argument_name argument context_with_function_matches context_with_matches)
       : Strict context (Pattern.App function_pattern argument_name) (Term.App function argument) context_with_matches
   .
-Arguments Strict context strict term context_with_matches.
+Arguments Strict context strict scrutinee context_with_matches.
 
-Fixpoint strict context pattern term : option Context.context :=
-  match pattern, term with
+Fixpoint strict context pattern scrutinee : option Context.context :=
+  match pattern, scrutinee with
   | Pattern.Ctr constructor_pattern, Term.Ctr constructor =>
       if Constructor.eq constructor_pattern constructor then Some context else None
   | Pattern.App function_pattern argument_name, Term.App function argument =>
@@ -51,15 +52,30 @@ Proof.
   - eapply Map.add_det; try reflexivity; try eassumption. apply IHS1. exact function_matched.
 Qed.
 
-Lemma strict_spec context pattern term
-  : Reflect.Option (Strict context pattern term) (strict context pattern term).
+Lemma strict_eq
+  c1 s1 t1 m1 (S : Strict c1 s1 t1 m1)
+  c2 (Ec : Map.Eq c1 c2)
+  s2 (Es : s1 = s2)
+  t2 (Et : t1 = t2)
+  m2 (Em : Map.Eq m1 m2)
+  : Strict c2 s2 t2 m2.
 Proof.
-  generalize dependent term. induction pattern; intros;
-  destruct term; try solve [constructor; intros t C; invert C].
+  subst. rename t2 into t. rename s2 into s. generalize dependent m2. generalize dependent c2. induction S; intros.
+  - constructor. eapply Map.eq_trans. 2: { eassumption. }
+    eapply Map.eq_trans. 2: { eassumption. } apply Map.eq_sym. exact Ec.
+  - econstructor. { apply IHS. { exact Ec. } apply Map.eq_refl. } { exact N. }
+    eapply Map.add_eq; try reflexivity; try eassumption. apply Map.eq_refl.
+Qed.
+
+Lemma strict_spec context pattern scrutinee
+  : Reflect.Option (Strict context pattern scrutinee) (strict context pattern scrutinee).
+Proof.
+  generalize dependent scrutinee. induction pattern; intros;
+  destruct scrutinee; try solve [constructor; intros t C; invert C].
   - unfold strict. destruct (Constructor.eq_spec constructor constructor0); constructor.
     + subst. constructor. apply Map.eq_refl.
     + intros t C. invert C. apply N. reflexivity.
-  - simpl strict. destruct (IHpattern term1) as [function_matches function_matched | N]. 2: {
+  - simpl strict. destruct (IHpattern scrutinee1) as [function_matches function_matched | N]. 2: {
       constructor. intros t C. invert C. apply N in function_matched as []. }
     destruct (Map.find_spec function_matches argument) as [duplicated F | N]. 2: {
       constructor. econstructor. { eassumption. } { intros [y F]. apply N in F as []. }
@@ -69,7 +85,7 @@ Proof.
     try eassumption. apply Map.eq_refl.
 Qed.
 
-Lemma in_strict {context strict term context_with_matches} (S : Strict context strict term context_with_matches) x
+Lemma in_strict {context strict scrutinee context_with_matches} (S : Strict context strict scrutinee context_with_matches) x
   : Map.In context_with_matches x <-> (BoundIn.Strict strict x \/ Map.In context x).
 Proof.
   generalize dependent x. induction S; intros.
@@ -83,6 +99,32 @@ Proof.
       destruct I as [B | I]; [invert B; [left; reflexivity |] |];
       right; apply IHS; [left | right]; assumption.
 Qed.
+
+Definition CompatibleStrict (context : Context.context) strict : Prop :=
+  forall x (I : Map.In context x) (B : BoundIn.Strict strict x), False.
+Arguments CompatibleStrict context strict/.
+
+Lemma compatible_strict_iff strict (WF : WellFormed.Strict strict) context
+  : CompatibleStrict context strict <->
+    exists scrutinee context_with_matches,
+    Strict context strict scrutinee context_with_matches.
+Proof.
+  split.
+  - induction WF; intros. { do 2 eexists. constructor. apply Map.eq_refl. }
+    edestruct IHWF as [scrutinee [context_with_matches IH]]; clear IHWF. {
+      intros x I B. eapply H. { exact I. } constructor. exact B. }
+    assert (N' : ~Map.In context_with_matches argument). { intro I.
+      eapply in_strict in I as [I | I]; [| | exact IH]. { apply N in I as []. } apply H in I as []. constructor. }
+    eexists (Term.App _ Term.Err). eexists. econstructor. { exact IH. } { exact N'. }
+    apply Map.add_overriding. intros v' F. eassert (I : Map.In _ _). { eexists. exact F. } apply N' in I as [].
+  - intros [scrutinee [context_with_matches S]] k I B. generalize dependent k. generalize dependent WF.
+    induction S; intros. { invert B. } invert B. { apply N. eapply in_strict. { exact S. } right. exact I. }
+    invert WF. eapply IHS. { exact curried_well_formed. } { exact I. } exact bound_earlier.
+Qed.
+
+Lemma compatible_strict_eq {c1 p1} (C : CompatibleStrict c1 p1) {c2} (Ec : Map.Eq c1 c2) {p2} (Ep : p1 = p2)
+  : CompatibleStrict c2 p2.
+Proof. subst. intros x I B. eapply C. { eapply Map.in_eq. { exact Ec. } exact I. } exact B. Qed.
 
 
 
@@ -102,10 +144,10 @@ Inductive StrictRef (context : Context.context) : Pattern.strict -> Term.term ->
         (Term.App function_cleaved (Term.Mov argument_name))
         context_with_matches
   .
-Arguments StrictRef context strict term cleaved context_with_matches.
+Arguments StrictRef context strict scrutinee cleaved context_with_matches.
 
-Fixpoint strict_ref context pattern term : option (Term.term * Context.context) :=
-  match pattern, term with
+Fixpoint strict_ref context pattern scrutinee : option (Term.term * Context.context) :=
+  match pattern, scrutinee with
   | Pattern.Ctr constructor_pattern, Term.Ctr constructor =>
       if Constructor.eq constructor_pattern constructor then Some (Term.Ctr constructor, context) else None
   | Pattern.App function_pattern argument_name, Term.App function argument =>
@@ -135,15 +177,33 @@ Proof.
     eapply Map.add_det; try reflexivity; eassumption.
 Qed.
 
-Lemma strict_ref_spec context pattern term
-  : Reflect.Option (fun pair => StrictRef context pattern term (fst pair) (snd pair)) (strict_ref context pattern term).
+Lemma strict_ref_eq
+  c1 s1 t1 y1 m1 (S : StrictRef c1 s1 t1 y1 m1)
+  c2 (Ec : Map.Eq c1 c2)
+  s2 (Es : s1 = s2)
+  t2 (Et : t1 = t2)
+  y2 (Ey : y1 = y2)
+  m2 (Em : Map.Eq m1 m2)
+  : StrictRef c2 s2 t2 y2 m2.
 Proof.
-  generalize dependent term. induction pattern; intros;
-  destruct term; try solve [constructor; intros t C; invert C].
+  subst. rename t2 into t. rename s2 into s. generalize dependent m2. generalize dependent c2. induction S; intros.
+  - constructor. eapply Map.eq_trans. 2: { eassumption. }
+    eapply Map.eq_trans. 2: { eassumption. } apply Map.eq_sym. exact Ec.
+  - econstructor. { apply IHS. { exact Ec. } apply Map.eq_refl. } { exact N. }
+    eapply Map.add_eq; try reflexivity; try eassumption. apply Map.eq_refl.
+Qed.
+
+Lemma strict_ref_spec context pattern scrutinee
+  : Reflect.Option
+    (fun pair => StrictRef context pattern scrutinee (fst pair) (snd pair))
+    (strict_ref context pattern scrutinee).
+Proof.
+  generalize dependent scrutinee. induction pattern; intros;
+  destruct scrutinee; try solve [constructor; intros t C; invert C].
   - unfold strict_ref. destruct (Constructor.eq_spec constructor constructor0); constructor.
     + subst. constructor. apply Map.eq_refl.
     + intros t C. invert C. apply N. reflexivity.
-  - simpl strict_ref. destruct (IHpattern term1) as [[cleaved function_matches] function_matched | N]. 2: {
+  - simpl strict_ref. destruct (IHpattern scrutinee1) as [[cleaved function_matches] function_matched | N]. 2: {
       constructor. intros t C. invert C. apply (N (_, _)) in function_matched as []. }
     destruct (Map.find_spec function_matches argument) as [duplicated F | N]. 2: {
       constructor. econstructor. { eassumption. } { intros [y F]. apply N in F as []. }
@@ -153,8 +213,8 @@ Proof.
     try eassumption. apply Map.eq_refl.
 Qed.
 
-Lemma in_strict_ref {context strict term cleaved context_with_matches}
-  (S : StrictRef context strict term cleaved context_with_matches) x
+Lemma in_strict_ref {context strict scrutinee cleaved context_with_matches}
+  (S : StrictRef context strict scrutinee cleaved context_with_matches) x
   : Map.In context_with_matches x <-> (BoundIn.Strict strict x \/ Map.In context x).
 Proof.
   generalize dependent x. induction S; intros.
@@ -169,23 +229,41 @@ Proof.
       right; apply IHS; [left | right]; assumption.
 Qed.
 
+Lemma compatible_strict_ref_iff strict (WF : WellFormed.Strict strict) context
+  : CompatibleStrict context strict <->
+    exists scrutinee cleaved context_with_matches,
+    StrictRef context strict scrutinee cleaved context_with_matches.
+Proof.
+  split.
+  - induction WF; intros. { do 3 eexists. constructor. apply Map.eq_refl. }
+    edestruct IHWF as [scrutinee [cleaved [context_with_matches IH]]]; clear IHWF. {
+      intros x I B. eapply H. { exact I. } constructor. exact B. }
+    assert (N' : ~Map.In context_with_matches argument). { intro I.
+      eapply in_strict_ref in I as [I | I]; [| | exact IH]. { apply N in I as []. } apply H in I as []. constructor. }
+    eexists (Term.App _ Term.Err). do 2 eexists. econstructor. { exact IH. } { exact N'. }
+    apply Map.add_overriding. intros v' F. eassert (I : Map.In _ _). { eexists. exact F. } apply N' in I as [].
+  - intros [scrutinee [cleaved [context_with_matches S]]] k I B. generalize dependent k. generalize dependent WF.
+    induction S; intros. { invert B. } invert B. { apply N. eapply in_strict_ref. { exact S. } right. exact I. }
+    invert WF. eapply IHS. { exact curried_well_formed. } { exact I. } exact bound_earlier.
+Qed.
+
 
 
 Variant MoveOrReference (context : Context.context) : Pattern.move_or_reference -> Term.term -> Context.context -> Prop :=
-  | Mov strict term context_with_matches (S : Strict context strict term context_with_matches)
-      : MoveOrReference context (Pattern.Mov strict) term context_with_matches
+  | Mov strict scrutinee context_with_matches (S : Strict context strict scrutinee context_with_matches)
+      : MoveOrReference context (Pattern.Mov strict) scrutinee context_with_matches
   | Ref
-      name term (lookup : Map.Find context name term)
-      strict old_context_with_matches cleaved (S : StrictRef context strict term cleaved old_context_with_matches)
+      name scrutinee (lookup : Map.Find context name scrutinee)
+      strict old_context_with_matches cleaved (S : StrictRef context strict scrutinee cleaved old_context_with_matches)
       context_with_matches (OW : Map.Overwrite name cleaved old_context_with_matches context_with_matches)
       : MoveOrReference context (Pattern.Ref strict) (Term.Ref name) context_with_matches
   .
-Arguments MoveOrReference context strict term context_with_matches.
+Arguments MoveOrReference context strict scrutinee context_with_matches.
 
 Example match_referenced_application ctor arg argn name (N : argn <> name)
   : let pattern := Pattern.Ref (Pattern.App (Pattern.Ctr ctor) argn) in
-    let term := Term.App (Term.Ctr ctor) arg in
-    let context := Map.overriding_add name term Map.empty in
+    let scrutinee := Term.App (Term.Ctr ctor) arg in
+    let context := Map.overriding_add name scrutinee Map.empty in
     let context_with_matches :=
       (* Note how each right-hand branch is turned into a `Mov` referencing the contents of the branch: *)
       Map.overriding_add name (Term.App (Term.Ctr ctor) (Term.Mov argn)) (
@@ -215,9 +293,10 @@ Qed.
 Example match_referenced_application_deep ctor arg1 arg2 arg1n arg2n name
   (N1 : arg1n <> name) (N2 : arg2n <> name) (N : arg2n <> arg1n)
   : let pattern := Pattern.Ref (Pattern.App (Pattern.App (Pattern.Ctr ctor) arg1n) arg2n) in
-    let term := Term.App (Term.App (Term.Ctr ctor) arg1) arg2 in
-    let context := Map.overriding_add name term Map.empty in
-    let context_with_matches := (* Note how each right-hand branch is turned into a `Mov` referencing the contents of the branch: *)
+    let scrutinee := Term.App (Term.App (Term.Ctr ctor) arg1) arg2 in
+    let context := Map.overriding_add name scrutinee Map.empty in
+    let context_with_matches :=
+      (* Note how each right-hand branch is turned into a `Mov` referencing the contents of the branch: *)
       Map.overriding_add name (Term.App (Term.App (Term.Ctr ctor) (Term.Mov arg1n)) (Term.Mov arg2n)) (
       Map.overriding_add arg1n arg1 (
       Map.overriding_add arg2n arg2 (
@@ -252,11 +331,11 @@ Proof.
       apply Map.find_singleton in F as [E ->]. apply N' in E as [].
 Qed.
 
-Definition move_or_reference context pattern term :=
+Definition move_or_reference context pattern scrutinee :=
   match pattern with
-  | Pattern.Mov s => strict context s term
+  | Pattern.Mov s => strict context s scrutinee
   | Pattern.Ref s =>
-      match term with
+      match scrutinee with
       | Term.Ref name =>
           match Map.find context name with
           | None => None
@@ -286,8 +365,23 @@ Proof.
     eapply Map.overwrite_det; try reflexivity; eassumption.
 Qed.
 
-Lemma in_move_or_reference {context move_or_reference term context_with_matches}
-  (MR : MoveOrReference context move_or_reference term context_with_matches) x
+Lemma move_or_reference_eq
+  c1 p1 t1 m1 (MR : MoveOrReference c1 p1 t1 m1)
+  c2 (Ec : Map.Eq c1 c2)
+  p2 (Ep : p1 = p2)
+  t2 (Et : t1 = t2)
+  m2 (Em : Map.Eq m1 m2)
+  : MoveOrReference c2 p2 t2 m2.
+Proof.
+  invert MR.
+  - constructor. eapply strict_eq; try reflexivity; eassumption.
+  - econstructor. { apply Ec. exact lookup. }
+    + eapply strict_ref_eq; try reflexivity; try eassumption. apply Map.eq_refl.
+    + eapply Map.overwrite_eq; try reflexivity; try eassumption. apply Map.eq_refl.
+Qed.
+
+Lemma in_move_or_reference {context move_or_reference scrutinee context_with_matches}
+  (MR : MoveOrReference context move_or_reference scrutinee context_with_matches) x
   : Map.In context_with_matches x <-> (BoundIn.MoveOrReference move_or_reference x \/ Map.In context x).
 Proof.
   invert MR.
@@ -297,13 +391,13 @@ Proof.
     split; (intros [B | I]; [left | right; exact I]). { constructor. exact B. } invert B. exact bound_in_strict.
 Qed.
 
-Lemma move_or_reference_spec context pattern term
-  : Reflect.Option (MoveOrReference context pattern term) (move_or_reference context pattern term).
+Lemma move_or_reference_spec context pattern scrutinee
+  : Reflect.Option (MoveOrReference context pattern scrutinee) (move_or_reference context pattern scrutinee).
 Proof.
   destruct pattern; cbn.
-  - cbn. destruct (strict_spec context strict0 term); constructor. { constructor. exact Y. }
+  - cbn. destruct (strict_spec context strict0 scrutinee); constructor. { constructor. exact Y. }
     intros x MR. invert MR. apply N in S as [].
-  - destruct term; try (constructor; intros m C; invert C).
+  - destruct scrutinee; try (constructor; intros m C; invert C).
     destruct (Map.find_spec context name). 2: { constructor. intros m C. invert C. apply N in lookup as []. }
     destruct (strict_ref_spec context strict0 x). 2: {
       constructor. intros m C. invert C. destruct (Map.find_det Y lookup). apply (N (_, _)) in S as []. }
@@ -311,24 +405,35 @@ Proof.
     apply Map.overwrite_overwrite. eapply in_strict_ref. { exact Y0. } right. eexists. exact Y.
 Qed.
 
+Variant CompatibleMoveOrReference context : Pattern.move_or_reference -> Prop :=
+  | CRef strict (strict_compatible : CompatibleStrict context strict) (* counterproductive to traverse an arbitrary graph of indirection *)
+      : CompatibleMoveOrReference context (Pattern.Ref strict)
+  | CMov strict (strict_compatible : CompatibleStrict context strict)
+      : CompatibleMoveOrReference context (Pattern.Mov strict)
+  .
+
+Lemma compatible_move_or_reference_eq {c1 p1} (C : CompatibleMoveOrReference c1 p1) {c2} (Ec : Map.Eq c1 c2) {p2} (Ep : p1 = p2)
+  : CompatibleMoveOrReference c2 p2.
+Proof. subst. invert C; constructor; eapply compatible_strict_eq; try reflexivity; eassumption. Qed.
+
 
 
 Variant Pattern (context : Context.context) : Pattern.pattern -> Term.term -> Context.context -> Prop :=
   | Nam
       name (N : forall (I : Map.In context name), False)
-      term context_with_matches (S : Map.Add name term context context_with_matches)
-      : Pattern context (Pattern.Nam name) term context_with_matches
+      scrutinee context_with_matches (S : Map.Add name scrutinee context context_with_matches)
+      : Pattern context (Pattern.Nam name) scrutinee context_with_matches
   | Pat
-      move_or_reference term context_with_matches (move_or_reference_matched
-        : MoveOrReference context move_or_reference term context_with_matches)
-      : Pattern context (Pattern.Pat move_or_reference) term context_with_matches
+      move_or_reference scrutinee context_with_matches (move_or_reference_matched
+        : MoveOrReference context move_or_reference scrutinee context_with_matches)
+      : Pattern context (Pattern.Pat move_or_reference) scrutinee context_with_matches
   .
-Arguments Pattern context pattern term context_with_matches.
+Arguments Pattern context pattern scrutinee context_with_matches.
 
-Definition pattern context patt term :=
+Definition pattern context patt scrutinee :=
   match patt with
-  | Pattern.Nam name => Map.disjoint_add name term context
-  | Pattern.Pat mor => move_or_reference context mor term
+  | Pattern.Nam name => Map.disjoint_add name scrutinee context
+  | Pattern.Pat mor => move_or_reference context mor scrutinee
   end.
 
 Lemma pattern_det
@@ -344,12 +449,40 @@ Proof.
   - eapply move_or_reference_det; try reflexivity; eassumption.
 Qed.
 
-Lemma pattern_spec context patt term
-  : Reflect.Option (Pattern context patt term) (pattern context patt term).
+Lemma pattern_eq
+  c1 p1 t1 m1 (P : Pattern c1 p1 t1 m1)
+  c2 (Ec : Map.Eq c1 c2)
+  p2 (Ep : p1 = p2)
+  t2 (Et : t1 = t2)
+  m2 (Em : Map.Eq m1 m2)
+  : Pattern c2 p2 t2 m2.
+Proof.
+  invert P.
+  - constructor. { intro I. eapply Map.in_eq in I. { apply N in I as []. } exact Ec. }
+    eapply Map.add_eq; try reflexivity; eassumption.
+  - constructor. eapply move_or_reference_eq; try reflexivity; try eassumption.
+Qed.
+
+Lemma pattern_spec context patt scrutinee
+  : Reflect.Option (Pattern context patt scrutinee) (pattern context patt scrutinee).
 Proof.
   destruct patt; cbn.
   - destruct (Map.find_spec context name); constructor. { intros m C. invert C. apply N. eexists. exact Y. }
     constructor. { intros [y F]. eapply N. exact F. } apply Map.add_overriding. cbn. intros. apply N in F as [].
-  - destruct (move_or_reference_spec context move_or_reference0 term); constructor. { constructor. exact Y. }
+  - destruct (move_or_reference_spec context move_or_reference0 scrutinee); constructor. { constructor. exact Y. }
     intros ctx C. invert C. apply N in move_or_reference_matched as [].
+Qed.
+
+Variant Compatible context : Pattern.pattern -> Prop :=
+  | CNam name (N : forall (I : Map.In context name), False)
+      : Compatible context (Pattern.Nam name)
+  | CPat move_or_reference (move_or_reference_compatible : CompatibleMoveOrReference context move_or_reference)
+      : Compatible context (Pattern.Pat move_or_reference)
+  .
+
+Lemma compatible_eq {c1 p1} (C : Compatible c1 p1) {c2} (Ec : Map.Eq c1 c2) {p2} (Ep : p1 = p2)
+  : Compatible c2 p2.
+Proof.
+  subst. invert C. { constructor. intro I. apply N. eapply Map.in_eq. { exact Ec. } exact I. }
+  constructor. eapply compatible_move_or_reference_eq; try reflexivity; eassumption.
 Qed.
