theories/NewNames.v
@@ -1,0 +1,111 @@
+From LinearCore Require
+  Map
+  Name
+  .
+From LinearCore Require Import
+  Invert
+  .
+
+
+
+Import Ascii.
+Definition underscore := "_"%char.
+
+Definition underscored name :=
+  match name with
+  | Name.Name head tail => Name.Name underscore (String.String head tail)
+  end.
+
+
+
+Definition in_ := @Map.in_.
+Arguments in_/ {T} m k.
+
+Axiom new_name : Map.set -> Name.name -> Name.name.
+Arguments new_name reserved orig_name.
+Extract Constant new_name =>
+  "let rec new_name' reserved name = if in_ name reserved then unbound' (underscored name) reserved else name in new_name'".
+
+Axiom not_in_new_name : forall reserved orig_name (I : Map.In reserved (new_name reserved orig_name)), False.
+Arguments not_in_new_name {reserved orig_name} I.
+
+Axiom new_name_det : forall r1 r2 (E : Map.Eq r1 r2) orig_name, new_name r1 orig_name = new_name r2 orig_name.
+Arguments new_name_det {r1 r2} E orig_name.
+
+
+
+Definition generate_acc acc reserved : Map.set -> Map.to Name.name :=
+  Map.fold (fun k _ acc => Map.overriding_add k (new_name (Map.set_union reserved (Map.domain acc)) k) acc) acc.
+Arguments generate_acc acc reserved names/.
+
+Definition generate : Map.set -> Map.set -> Map.to Name.name := generate_acc Map.empty.
+Arguments generate reserved names/.
+
+
+
+Lemma in_generate_acc acc reserved names k :
+  Map.In (generate_acc acc reserved names) k <-> (Map.In names k \/ Map.In acc k).
+Proof.
+  cbn. unfold Map.fold. rewrite MapCore.fold_spec. assert (Iff :
+    ((exists v, Map.Find names k v) \/ (exists v, Map.Find acc k v)) <->
+    ((exists v, SetoidList.InA MapCore.eq_key_elt (k, v) (MapCore.bindings names)) \/ (exists v, Map.Find acc k v))). {
+    split; (intros [[v F] | [v F]]; [left | right]; exists v; [| exact F]); apply MapCore.bindings_spec1; exact F. }
+  rewrite Iff; clear Iff. remember (MapCore.bindings names) as b eqn:Eb; clear names Eb; rename b into names.
+  generalize dependent k. generalize dependent reserved. generalize dependent acc.
+  induction names as [| [k v] tail]; intros. {
+    cbn. split. { intros [v F]. right. exists v. exact F. }
+    intros [[v F] | [v F]]. 2: { exists v. exact F. } invert F. }
+  rename k0 into x. cbn. rewrite IHtail; clear IHtail. split; intros [[y F] | [y F]].
+  - left. exists y. right. exact F.
+  - apply Map.find_overriding_add in F as [[-> ->] | [N F]]. 2: { right. exists y. exact F. }
+    left. exists v. left. split; reflexivity.
+  - invert F. 2: { left. eexists. eassumption. }
+    destruct H0; cbn in *; subst. right. eexists. apply Map.find_overriding_add. left. split; reflexivity.
+  - right. destruct (Name.spec x k); subst; eexists; apply Map.find_overriding_add;
+    [left | right]. { split; reflexivity. } split; eassumption.
+Qed.
+
+Lemma not_in_generate_acc
+  reserved x (R : Map.In reserved x)
+  acc (N : forall k (R : Map.In reserved k) (A : Map.InRange acc k), False)
+  names (G : Map.InRange (generate_acc acc reserved names) x)
+  : False.
+Proof.
+  cbn in G. destruct G as [y G]. unfold Map.fold in G. rewrite MapCore.fold_spec in G.
+  remember (MapCore.bindings names) as b eqn:Eb; clear names Eb; rename b into names.
+  generalize dependent y. generalize dependent acc. generalize dependent x. generalize dependent reserved.
+  induction names as [| [k v] tail]; intros. { cbn in *. destruct R. eapply N; eexists; eassumption. }
+  simpl List.fold_left in G. apply IHtail in G as []; clear IHtail. { exact R. }
+  intros z Rz I. destruct I as [z' F]. apply Map.find_overriding_add in F as [[-> ->] | [Nz F]].
+  - eapply not_in_new_name. apply Map.in_overriding_union. left. exact Rz.
+  - eapply N. { exact Rz. } eexists. exact F.
+Qed.
+
+Lemma not_in_generate
+  reserved k (R : Map.In reserved k)
+  names (G : Map.InRange (generate reserved names) k)
+  : False.
+Proof. eapply not_in_generate_acc; try eassumption. intros x I [y C]. invert C. Qed.
+
+Lemma generate_acc_det {a1 a2} (Ea : Map.Eq a1 a2) {r1 r2} (Er : Map.Eq r1 r2) {n1 n2} (En : Map.Eq n1 n2)
+  : Map.Eq (generate_acc a1 r1 n1) (generate_acc a2 r2 n2).
+Proof.
+  intros x y. unfold generate. unfold generate_acc. unfold Map.fold.
+  repeat rewrite MapCore.fold_spec. apply Map.bindings_eq in En.
+  remember (MapCore.bindings n1) as b1 eqn:E1; clear n1 E1; rename b1 into n1.
+  remember (MapCore.bindings n2) as b2 eqn:E2; clear n2 E2; rename b2 into n2.
+  subst. rename n2 into names. generalize dependent y. generalize dependent x. generalize dependent r2.
+  generalize dependent r1. generalize dependent a2. generalize dependent a1.
+  induction names as [| [k v] tail IH]; intros; cbn in *. { apply Ea. }
+  apply IH. 2: { exact Er. } intros. repeat rewrite Map.find_overriding_add. rewrite Ea.
+  erewrite new_name_det. { reflexivity. } cbn. intros. repeat rewrite Map.find_iff.
+  repeat rewrite Map.find_overriding_union. destruct (Map.find_spec r1 k1).
+  - apply Er in Y. apply Map.find_iff in Y. rewrite Y. reflexivity.
+  - destruct (Map.find_spec r2 k1). { apply Er in Y. apply N in Y as []. }
+    repeat rewrite <- Map.find_iff. fold (Map.domain a1). fold (Map.domain a2).
+    repeat rewrite Map.find_domain. erewrite Map.in_eq. { reflexivity. } assumption.
+Qed.
+
+Lemma generate_det {r1 r2} (Er : Map.Eq r1 r2) {n1 n2} (En : Map.Eq n1 n2)
+  : Map.Eq (generate r1 n1) (generate r2 n2).
+Proof. apply generate_acc_det; try assumption. apply Map.eq_refl. Qed.
