theories/Reflect.v
@@ -22,41 +22,41 @@ Variant Option {T} (P : T -> Prop) : option T -> Prop :=
 
 
 
-Lemma bool_iff P b (R : Bool P b)
+Lemma bool_iff {P b} (R : Bool P b)
   : P <-> b = true.
 Proof. invert R; split; intro C; try tauto. discriminate C. Qed.
 
-Lemma bool_niff P b (R : Bool P b)
+Lemma bool_niff {P b} (R : Bool P b)
   : ~P <-> b = false.
 Proof. invert R; split; intro C; try tauto. discriminate C. Qed.
 
 Lemma bool_eq
-  Q P (E : P <-> Q) b
+  {Q P} (E : P <-> Q) b
   : Bool P b <-> Bool Q b.
 Proof. split; intro R; (destruct R; constructor; [apply E; exact Y |]); intro C; apply N0; apply E; exact C. Qed.
 
 Lemma bool_det
-  P p (Rp : Bool P p)
-  Q q (Rq : Bool Q q)
+  {P p} (Rp : Bool P p)
+  {Q q} (Rq : Bool Q q)
   (E : P <-> Q)
   : p = q.
 Proof. invert Rp; invert Rq; tauto. Qed.
 
 Lemma and
-  P p (Rp : Bool P p)
-  Q q (Rq : Bool Q q)
+  {P p} (Rp : Bool P p)
+  {Q q} (Rq : Bool Q q)
   : Bool (P /\ Q) (p && q).
 Proof. invert Rp; invert Rq; constructor; tauto. Qed.
 
 Lemma or
-  P p (Rp : Bool P p)
-  Q q (Rq : Bool Q q)
+  {P p} (Rp : Bool P p)
+  {Q q} (Rq : Bool Q q)
   : Bool (P \/ Q) (p || q).
 Proof. invert Rp; invert Rq; constructor; tauto. Qed.
 
 
 
 Lemma opt_eq {T}
-  Q P (E : forall x : T, P x <-> Q x) opt
+  {Q P} (E : forall x : T, P x <-> Q x) opt
   : Option P opt <-> Option Q opt.
 Proof. split; intro R; (destruct R; constructor; [apply E; assumption |]); intros x C; eapply N0; apply E; exact C. Qed.
