theories/Rename.v
@@ -1,0 +1,301 @@
+From LinearCore Require
+  Name
+  Term
+  UsedIn
+  .
+From LinearCore Require Import
+  Invert
+  .
+
+
+
+Inductive Strict (lookup : Map.to Name.name) : Pattern.strict -> Pattern.strict -> Prop :=
+  | SCtr ctor
+      : Strict lookup (Pattern.Ctr ctor) (Pattern.Ctr ctor)
+  | SApp
+      curried renamed_curried (rename_curried : Strict lookup curried renamed_curried)
+      argument renamed_argument (rename_argument : Map.Find lookup argument renamed_argument)
+      : Strict lookup (Pattern.App curried argument) (Pattern.App renamed_curried renamed_argument)
+  .
+Arguments Strict lookup strict renamed_strict.
+
+Fixpoint strict lookup s :=
+  match s with
+  | Pattern.Ctr ctor => Some s
+  | Pattern.App curried argument =>
+      match strict lookup curried with None => None | Some renamed_curried =>
+        option_map (Pattern.App renamed_curried) (Map.find lookup argument)
+      end
+  end.
+
+Lemma strict_spec lookup s
+  : Reflect.Option (Strict lookup s) (strict lookup s).
+Proof.
+  induction s; cbn in *. { constructor. constructor. }
+  destruct IHs. 2: { constructor. intros t S. invert S. apply N in rename_curried as []. }
+  destruct (Map.find_spec lookup argument); constructor. { constructor; assumption. }
+  intros s' S. invert S. apply N in rename_argument as [].
+Qed.
+
+Lemma strict_det
+  {l1 s1 r1} (S1 : Strict l1 s1 r1)
+  {l2} (El : Map.Eq l1 l2)
+  {s2} (Es : s1 = s2)
+  {r2} (S2 : Strict l2 s2 r2)
+  : r1 = r2.
+Proof.
+  subst. generalize dependent r2. generalize dependent l2.
+  induction S1; intros; invert S2. { reflexivity. }
+  f_equal. { eapply IHS1. { exact El. } exact rename_curried. }
+  eapply Map.find_det; try eassumption. apply El. assumption.
+Qed.
+
+
+
+Variant MoveOrReference lookup : Pattern.move_or_reference -> Pattern.move_or_reference -> Prop :=
+  | MMov strict renamed_strict (rename_strict : Strict lookup strict renamed_strict)
+      : MoveOrReference lookup (Pattern.Mov strict) (Pattern.Mov renamed_strict)
+  | MRef strict renamed_strict (rename_strict : Strict lookup strict renamed_strict)
+      : MoveOrReference lookup (Pattern.Ref strict) (Pattern.Ref renamed_strict)
+  .
+
+Definition move_or_reference lookup mr :=
+  match mr with
+  | Pattern.Mov s => option_map Pattern.Mov (strict lookup s)
+  | Pattern.Ref s => option_map Pattern.Ref (strict lookup s)
+  end.
+
+Lemma move_or_reference_spec lookup mr
+  : Reflect.Option (MoveOrReference lookup mr) (move_or_reference lookup mr).
+Proof.
+  destruct mr; cbn; (destruct (strict_spec lookup strict0); constructor; [constructor; exact Y |]);
+  intros s M; invert M; apply N in rename_strict as [].
+Qed.
+
+Lemma move_or_reference_det
+  {l1 mr1 r1} (MR1 : MoveOrReference l1 mr1 r1)
+  {l2} (El : Map.Eq l1 l2)
+  {mr2} (Emr : mr1 = mr2)
+  {r2} (MR2 : MoveOrReference l2 mr2 r2)
+  : r1 = r2.
+Proof. invert MR1; invert MR2; f_equal; eapply strict_det; try reflexivity; eassumption. Qed.
+
+
+
+Variant Pattern lookup : Pattern.pattern -> Pattern.pattern -> Prop :=
+  | Nam name renamed (rename_name : Map.Find lookup name renamed)
+      : Pattern lookup (Pattern.Nam name) (Pattern.Nam renamed)
+  | Pat move_or_reference renamed_move_or_reference
+      (rename_move_or_reference : MoveOrReference lookup move_or_reference renamed_move_or_reference)
+      : Pattern lookup (Pattern.Pat move_or_reference) (Pattern.Pat renamed_move_or_reference)
+  .
+
+Definition pattern lookup p :=
+  match p with
+  | Pattern.Nam name => option_map Pattern.Nam (Map.find lookup name)
+  | Pattern.Pat mr => option_map Pattern.Pat (move_or_reference lookup mr)
+  end.
+
+Lemma pattern_spec lookup p
+  : Reflect.Option (Pattern lookup p) (pattern lookup p).
+Proof.
+  destruct p; cbn in *.
+  - destruct (Map.find_spec lookup name); constructor. { constructor. exact Y. }
+    intros p P. invert P. apply N in rename_name as [].
+  - destruct (move_or_reference_spec lookup move_or_reference0); constructor. { constructor. exact Y. }
+    intros p P. invert P. apply N in rename_move_or_reference as [].
+Qed.
+
+Lemma pattern_det
+  {l1 p1 r1} (P1 : Pattern l1 p1 r1)
+  {l2} (El : Map.Eq l1 l2)
+  {p2} (Ep : p1 = p2)
+  {r2} (P2 : Pattern l2 p2 r2)
+  : r1 = r2.
+Proof.
+  invert P1; invert P2; f_equal. { eapply Map.find_det. { eassumption. } apply El. assumption. }
+  eapply move_or_reference_det; try reflexivity; eassumption.
+Qed.
+
+
+
+Inductive Term (lookup : Map.to Name.name) : Term.term -> Term.term -> Prop :=
+  | Err
+      : Term lookup Term.Err Term.Err
+  | Typ
+      : Term lookup Term.Typ Term.Typ
+  | Prp
+      : Term lookup Term.Prp Term.Prp
+  | Ctr ctor
+      : Term lookup (Term.Ctr ctor) (Term.Ctr ctor) (* constructor names live in a different universe *)
+  | Mov x y (F : Map.Find lookup x y)
+      : Term lookup (Term.Mov x) (Term.Mov y)
+  | Ref x y (F : Map.Find lookup x y)
+      : Term lookup (Term.Ref x) (Term.Ref y)
+  | App
+      function renamed_function (function_renaming : Term lookup function renamed_function)
+      argument renamed_argument (argument_renaming : Term lookup argument renamed_argument)
+      : Term lookup (Term.App function argument) (Term.App renamed_function renamed_argument)
+  | For
+      type renamed_type (type_renaming : Term lookup type renamed_type)
+      variable unshadowed (not_shadowed : Map.OverwriteIfPresent variable variable lookup unshadowed)
+      body renamed_body (body_renaming : Term unshadowed body renamed_body)
+      : Term lookup (Term.For variable type body) (Term.For variable renamed_type renamed_body)
+  | Cas
+      other_cases renamed_other_cases (other_cases_renaming : Term lookup other_cases renamed_other_cases)
+      pattern bound_in_pattern (find_pattern_bindings : Map.Reflect (BoundIn.Pattern pattern) bound_in_pattern)
+      pattern_to_self (pattern_idem : Map.ToSelf bound_in_pattern pattern_to_self)
+      unshadowed (not_shadowed : Map.BulkOverwrite pattern_to_self lookup unshadowed)
+      body_if_match renamed_body_if_match (body_if_match_renaming : Term unshadowed body_if_match renamed_body_if_match)
+      : Term lookup
+        (Term.Cas pattern body_if_match other_cases)
+        (Term.Cas pattern renamed_body_if_match renamed_other_cases)
+  .
+Arguments Term lookup term renamed.
+
+
+
+Lemma eq {l1 t1 y1} (R1 : Term l1 t1 y1)
+  {l2} (El : Map.Eq l1 l2)
+  {t2} (Et : t1 = t2)
+  {y2} (Ey : y1 = y2)
+  : Term l2 t2 y2.
+Proof.
+  subst. rename t2 into t. rename y2 into y. generalize dependent l2. induction R1; intros.
+  - constructor.
+  - constructor.
+  - constructor.
+  - constructor.
+  - constructor. apply El. exact F.
+  - constructor. apply El. exact F.
+  - constructor; [apply IHR1_1 | apply IHR1_2]; exact El.
+  - econstructor. { apply IHR1_1. exact El. } 2: { exact R1_2. }
+    eapply Map.overwrite_if_present_eq; try reflexivity; try eassumption. apply Map.eq_refl.
+  - econstructor; try eassumption. { apply IHR1_1. exact El. }
+    eapply Map.bulk_overwrite_eq; try eassumption; apply Map.eq_refl.
+Qed.
+
+
+
+(* TODO: Grammar: should this have an `e`? I'm leaning toward yes. *)
+Definition RenameableTerm (lookup : Map.to Name.name) term : Prop :=
+  forall x (U : UsedIn.Term term x), Map.In lookup x.
+Arguments RenameableTerm lookup term/.
+
+Lemma renameable_term lookup term :
+  (exists renamed, Term lookup term renamed) <-> RenameableTerm lookup term.
+Proof.
+  cbn. split.
+  - intros [renamed R]; intros. induction R.
+    + invert U.
+    + invert U.
+    + invert U.
+    + invert U.
+    + invert U. eexists. exact F.
+    + invert U. eexists. exact F.
+    + invert U; [apply IHR1 | apply IHR2]; assumption.
+    + invert U. { apply IHR1. assumption. } specialize (IHR2 used_in_body) as [y IH].
+      apply not_shadowed in IH as [[-> ->] | [N F]]. { contradiction not_shadowed0. reflexivity. } eexists. exact F.
+    + invert U. 2: { apply IHR1. exact used_in_another_case. } specialize (IHR2 used_in_body) as [y IH].
+      apply not_shadowed in IH as [F | [N F]]. 2: { eexists. exact F. }
+      apply pattern_idem in F as [I ->]. apply find_pattern_bindings in I. apply not_shadowed0 in I as [].
+  - intros I. generalize dependent lookup. induction term; intros.
+    + eexists. constructor.
+    + eexists. constructor.
+    + eexists. constructor.
+    + eexists. constructor.
+    + edestruct I as [y F]. { constructor. } eexists. constructor. exact F.
+    + edestruct I as [y F]. { constructor. } eexists. constructor. exact F.
+    + edestruct IHterm1 as [rf IHf]. { intros. apply I. apply UsedIn.ApF. exact U. }
+      edestruct IHterm2 as [ra IHa]. { intros. apply I. apply UsedIn.ApA. exact U. }
+      eexists. constructor; [exact IHf | exact IHa].
+    + edestruct IHterm1 as [rt IHt]. { intros. apply I. apply UsedIn.FoT. exact U. }
+      edestruct IHterm2 as [rb IHb]. 2: {
+        eexists. econstructor; try eassumption. apply Map.overwrite_if_present_overwrite. }
+      intros. eapply Map.in_overwrite_if_present. { apply Map.overwrite_if_present_overwrite. }
+      destruct (Name.spec x variable); [left | right]. { exact Y. } apply I. apply UsedIn.FoB; assumption.
+    + edestruct IHterm2 as [ro IHo]. { intros. apply I. apply UsedIn.CaO. exact U. }
+      edestruct IHterm1 as [rb IHb]. 2: {
+        eexists. econstructor; try eassumption. { apply BoundIn.pattern_spec. } { apply Map.to_self_to_self. }
+        apply Map.bulk_overwrite_bulk_overwrite. }
+      intros. eapply Map.in_bulk_overwrite. { apply Map.bulk_overwrite_bulk_overwrite. }
+      rewrite Map.in_to_self. destruct (Map.in_spec (BoundIn.pattern pattern0) x); [left | right]. { exact Y. }
+      split. { exact N. } apply I. apply UsedIn.CaB. 2: { exact U. }
+      intro B. apply N. apply BoundIn.pattern_spec. exact B.
+Qed.
+
+
+
+Fixpoint term lookup t :=
+  match t with
+  | Term.Mov name => option_map Term.Mov (Map.find lookup name)
+  | Term.Ref name => option_map Term.Ref (Map.find lookup name)
+  | Term.App function argument =>
+      match term lookup function with None => None | Some renamed_function =>
+        option_map (Term.App renamed_function) (term lookup argument)
+      end
+  | Term.For variable type body =>
+      match term lookup type with None => None | Some renamed_type =>
+        let unshadowed := Map.overwrite variable variable lookup in
+        option_map (Term.For variable renamed_type) (term unshadowed body)
+      end
+  | Term.Cas pattern body_if_match other_cases =>
+      match term lookup other_cases with None => None | Some renamed_other_cases =>
+        let unshadowed := Map.bulk_overwrite (Map.to_self (BoundIn.pattern pattern)) lookup in
+        option_map (fun renamed_body_if_match => Term.Cas pattern renamed_body_if_match renamed_other_cases)
+          (term unshadowed body_if_match)
+      end
+  | _ => Some t
+  end.
+
+Lemma term_spec lookup t
+  : Reflect.Option (Term lookup t) (term lookup t).
+Proof.
+  generalize dependent lookup. induction t; intros; cbn in *; try solve [repeat constructor].
+  - destruct (Map.find_spec lookup name); constructor. { constructor. exact Y. }
+    intros t C. invert C. apply N in F as [].
+  - destruct (Map.find_spec lookup name); constructor. { constructor. exact Y. }
+    intros t C. invert C. apply N in F as [].
+  - destruct (IHt1 lookup). 2: { constructor. intros t C. invert C. apply N in function_renaming as []. }
+    destruct (IHt2 lookup); constructor. { constructor; assumption. }
+    intros t C. invert C. apply N in argument_renaming as [].
+  - destruct (IHt1 lookup). 2: { constructor. intros t C. invert C. apply N in type_renaming as []. }
+    destruct (IHt2 (Map.overriding_add variable variable lookup)); constructor. {
+      econstructor; try eassumption. apply Map.overwrite_if_present_overwrite. }
+    intros t C. invert C. eapply N. eapply eq; try reflexivity; try eassumption.
+    eapply Map.overwrite_if_present_det; try reflexivity; try eassumption. { apply Map.eq_refl. }
+    apply Map.overwrite_if_present_overwrite.
+  - destruct (IHt2 lookup). 2: { constructor. intros t C. invert C. apply N in other_cases_renaming as []. }
+    fold (Map.to_self (BoundIn.pattern pattern0)).
+    destruct (IHt1 (Map.overriding_union (Map.to_self (BoundIn.pattern pattern0)) lookup)); constructor. {
+      econstructor; try eassumption. { apply BoundIn.pattern_spec. } { apply Map.to_self_to_self. }
+      apply Map.bulk_overwrite_bulk_overwrite. }
+    intros t R. invert R. eapply N. eapply eq; try reflexivity. { exact body_if_match_renaming. }
+    eapply Map.bulk_overwrite_det. { exact not_shadowed. } 3: { apply Map.bulk_overwrite_bulk_overwrite. }
+    2: { apply Map.eq_refl. } eapply Map.to_self_det; try eassumption. 2: { apply Map.to_self_to_self. }
+    intros x' y'. split; intro F; (eassert (I : Map.In _ _); [eexists; exact F |]).
+    + eapply find_pattern_bindings in I. apply BoundIn.pattern_spec in I. destruct I as [[] I]. destruct y'. exact I.
+    + apply BoundIn.pattern_spec in I. apply find_pattern_bindings in I. destruct I as [[] I]. destruct y'. exact I.
+Qed.
+
+Lemma term_det
+  {l1 t1 r1} (T1 : Term l1 t1 r1)
+  {l2} (El : Map.Eq l1 l2)
+  {t2} (Et : t1 = t2)
+  {r2} (T2 : Term l2 t2 r2)
+  : r1 = r2.
+Proof.
+  subst. generalize dependent r2. generalize dependent l2. induction T1; intros; invert T2; try reflexivity.
+  - f_equal. eapply Map.find_det. { eassumption. } apply El. assumption.
+  - f_equal. eapply Map.find_det. { eassumption. } apply El. assumption.
+  - f_equal; [eapply IHT1_1 | eapply IHT1_2]; eassumption.
+  - f_equal. { eapply IHT1_1; eassumption. } eapply IHT1_2. 2: { eassumption. }
+    eapply Map.overwrite_if_present_det; try reflexivity; eassumption.
+  - f_equal. 2: { eapply IHT1_1; eassumption. } eapply IHT1_2. 2: { eassumption. }
+    eapply Map.bulk_overwrite_det; try reflexivity; try eassumption.
+    eapply Map.to_self_det; try eassumption. intros x [].
+    split; intro F; (eassert (I : Map.In _ _); [eexists; exact F |]);
+    [apply find_pattern_bindings in I | apply find_pattern_bindings0 in I];
+    [apply find_pattern_bindings0 in I | apply find_pattern_bindings in I];
+    destruct I as [[] F']; exact F'.
+Qed.
