theories/Shape.v
@@ -1,0 +1,21 @@
+From LinearCore Require
+  Term
+  .
+
+
+
+Variant shape : Set :=
+  | Resource
+  | Function
+  .
+
+
+
+Inductive Shape : shape -> Term.term -> Prop :=
+  | Ctr ctor
+      : Shape Resource (Term.Ctr ctor)
+  | App curried (curried_resource : Shape Resource curried) argument
+      : Shape Resource (Term.App curried argument)
+  | Cas pattern body_if_match other_cases
+      : Shape Function (Term.Cas pattern body_if_match other_cases)
+  .
