theories/SmallStep.v
@@ -1,0 +1,159 @@
+From LinearCore Require
+  Context
+  Match
+  NewNames
+  Rename
+  Shape
+  Term
+  UsedIn
+  .
+From LinearCore Require Import
+  Invert
+  .
+
+
+
+Inductive Step (context : Context.context) : Term.term -> Context.context -> Term.term -> Prop :=
+  | Mov
+      name term (lookup : Map.Find context name term)
+      context_without_name (no_contraction : Map.Remove name context context_without_name)
+      : Step context (Term.Mov name) context_without_name term
+  | Ref
+      self term (lookup : Map.Find context self term)
+      context_without_self (remove_self_from_context : Map.Remove self context context_without_self)
+      stepped updated_context_without_self (step_in_context
+        : Step context_without_self term updated_context_without_self stepped)
+      (not_overwriting_self : forall (I : Map.In updated_context_without_self self), False)
+      context_updated_in_place (update
+        : Map.Add self stepped updated_context_without_self context_updated_in_place)
+      : Step context (Term.Ref self) context_updated_in_place (Term.Ref self)
+  | ApM
+      pattern (compatible_names : Match.Compatible context pattern)
+      scrutinee (safe_names : forall x (U : UsedIn.Term scrutinee x) (B : BoundIn.Pattern pattern x), False)
+      context_with_matches (matched
+        : Match.Pattern context pattern scrutinee context_with_matches)
+      body_if_match other_cases
+      : Step context
+        (Term.App (Term.Cas pattern body_if_match other_cases) scrutinee)
+        context_with_matches body_if_match
+  | ApS
+      pattern (compatible_names : Match.Compatible context pattern)
+      scrutinee (safe_names : forall x (U : UsedIn.Term scrutinee x) (B : BoundIn.Pattern pattern x), False)
+      (no_match : forall context_with_matches (M : Match.Pattern context pattern scrutinee context_with_matches), False)
+      updated_context reduced_scrutinee (reduce_scrutinee : Step context scrutinee updated_context reduced_scrutinee)
+      body_if_match other_cases
+      : Step context
+        (Term.App (Term.Cas pattern body_if_match other_cases) scrutinee)
+        updated_context
+        (Term.App (Term.Cas pattern body_if_match other_cases) reduced_scrutinee)
+  | ApN
+      pattern (compatible_names : Match.Compatible context pattern)
+      scrutinee (safe_names : forall x (U : UsedIn.Term scrutinee x) (B : BoundIn.Pattern pattern x), False)
+      (no_match : forall context_with_matches (M : Match.Pattern context pattern scrutinee context_with_matches), False)
+      shape (scrutinee_reduced : Shape.Shape shape scrutinee) body_if_match other_cases
+      : Step
+        context (Term.App (Term.Cas pattern body_if_match other_cases) scrutinee)
+        context (Term.App other_cases scrutinee)
+  | ApR
+      pattern scrutinee (not_yet_safe_to_match
+        : ~Match.Compatible context pattern \/ exists x, UsedIn.Term scrutinee x /\ BoundIn.Pattern pattern x)
+      body_if_match other_cases other_used (all_other_used_names
+        (* Note that this removes already bound terms, since `UsedIn` won't shadow: *)
+        : Map.Reflect (UsedIn.Term (Term.App (Term.Cas pattern body_if_match other_cases) scrutinee)) other_used)
+      reserved (union_into_reserved : Map.Union (Map.domain context) other_used reserved)
+      new_names (generate_new_names : NewNames.generate reserved (BoundIn.pattern pattern) = new_names)
+      renamed_pattern (rename_pattern : Rename.Pattern new_names pattern renamed_pattern)
+      map_body_if_match (overwrite_body_if_match
+        : Map.BulkOverwrite new_names (Map.to_self (UsedIn.term body_if_match)) map_body_if_match)
+      renamed_body_if_match (rename_body_if_match
+        : Rename.Term map_body_if_match body_if_match renamed_body_if_match)
+      map_other_cases (overwrite_other_cases
+        : Map.BulkOverwrite new_names (Map.to_self (UsedIn.term other_cases)) map_other_cases)
+      renamed_other_cases (rename_other_cases
+        : Rename.Term map_other_cases other_cases renamed_other_cases)
+      : Step
+        context (Term.App (Term.Cas pattern body_if_match other_cases) scrutinee)
+        context (Term.App (Term.Cas renamed_pattern renamed_body_if_match renamed_other_cases) scrutinee)
+    .
+Arguments Step context term updated_context updated_term.
+
+
+
+Theorem shapes_cant_step
+  {shape term} (shaped : Shape.Shape shape term)
+  {context updated_context updated_term} (step : Step context term updated_context updated_term)
+  : False.
+Proof.
+  generalize dependent updated_term. generalize dependent updated_context. generalize dependent context.
+  induction shaped; intros; invert step; invert shaped.
+Qed.
+
+
+
+Theorem step_det
+  {c1 t1 c1' t1'} (S1 : Step c1 t1 c1' t1')
+  {c2} (Ec : Map.Eq c1 c2)
+  {t2} (Et : t1 = t2)
+  {c2' t2'} (S2 : Step c2 t2 c2' t2')
+  : Map.Eq c1' c2' /\ t1' = t2'.
+Proof.
+  subst. rename t2 into t. generalize dependent t2'. generalize dependent c2'. generalize dependent c2.
+  induction S1; intros.
+  - invert S2. apply Ec in lookup0. destruct (Map.find_det lookup lookup0). split. 2: { reflexivity. }
+    eapply Map.remove_det; try reflexivity; eassumption.
+  - invert S2. split. 2: { reflexivity. } assert (RD :=
+      Map.remove_det remove_self_from_context eq_refl Ec remove_self_from_context0).
+    specialize (IHS1 _ RD). apply Ec in lookup0. destruct (Map.find_det lookup lookup0).
+    specialize (IHS1 _ _ step_in_context) as [Eu <-]. eapply Map.add_det; try reflexivity; eassumption.
+  - invert S2.
+    + split. 2: { reflexivity. } eapply Match.pattern_det; try reflexivity; eassumption.
+    + contradiction (no_match context_with_matches).
+      eapply Match.pattern_eq; try reflexivity; try eassumption; apply Map.eq_refl.
+    + contradiction (no_match context_with_matches).
+      eapply Match.pattern_eq; try reflexivity; try eassumption; apply Map.eq_refl.
+    + destruct not_yet_safe_to_match as [N | N].
+      * contradiction N. eapply Match.compatible_eq; try reflexivity; eassumption.
+      * destruct N as [x [U B]]. edestruct safe_names. { exact U. } exact B.
+  - invert S2.
+    + contradiction (no_match c2'). eapply Match.pattern_eq; try reflexivity; try eassumption. 2: { apply Map.eq_refl. }
+      apply Map.eq_sym. exact Ec.
+    + edestruct IHS1 as [Ec' E]. { exact Ec. } { exact reduce_scrutinee. } subst reduced_scrutinee0.
+      split. { exact Ec'. } reflexivity.
+    + eapply shapes_cant_step in scrutinee_reduced as []. eassumption.
+    + destruct not_yet_safe_to_match as [N | N].
+      * contradiction N. eapply Match.compatible_eq; try reflexivity; eassumption.
+      * destruct N as [x [U B]]. edestruct safe_names. { exact U. } exact B.
+  - invert S2.
+    + contradiction (no_match c2'). eapply Match.pattern_eq; try reflexivity; try eassumption. 2: { apply Map.eq_refl. }
+      apply Map.eq_sym. exact Ec.
+    + eapply shapes_cant_step in scrutinee_reduced as []. eassumption.
+    + split. { exact Ec. } reflexivity.
+    + destruct not_yet_safe_to_match as [N | N].
+      * contradiction N. eapply Match.compatible_eq; try reflexivity; eassumption.
+      * destruct N as [x [U B]]. edestruct safe_names. { exact U. } exact B.
+  - invert S2.
+    + destruct not_yet_safe_to_match as [N | N].
+      * contradiction N. eapply Match.compatible_eq; try reflexivity; try eassumption. apply Map.eq_sym. assumption.
+      * destruct N as [x [U B]]. edestruct safe_names. { exact U. } exact B.
+    + destruct not_yet_safe_to_match as [N | N].
+      * contradiction N. eapply Match.compatible_eq; try reflexivity; try eassumption. apply Map.eq_sym. assumption.
+      * destruct N as [x [U B]]. edestruct safe_names. { exact U. } exact B.
+    + destruct not_yet_safe_to_match as [N | N].
+      * contradiction N. eapply Match.compatible_eq; try reflexivity; try eassumption. apply Map.eq_sym. assumption.
+      * destruct N as [x [U B]]. edestruct safe_names. { exact U. } exact B.
+    + split. { exact Ec. } f_equal. assert (Eng : Map.Eq (NewNames.generate reserved (BoundIn.pattern pattern))
+        (NewNames.generate reserved0 (BoundIn.pattern pattern))). {
+        apply NewNames.generate_det. 2: { apply Map.eq_refl. }
+        eapply Map.union_det; try eassumption.
+        * split; intro F; apply Map.find_domain; apply Map.find_domain in F;
+          eapply Map.in_eq; try exact F. { apply Map.eq_sym. exact Ec. } exact Ec.
+        * split; intro F; (eassert (I : Map.In _ _); [eexists; exact F |]);
+          [apply all_other_used_names in I | apply all_other_used_names0 in I];
+          [apply all_other_used_names0 in I | apply all_other_used_names in I];
+          destruct I as [[] I]; destruct v; exact I. }
+      f_equal. { eapply Rename.pattern_det; try reflexivity; eassumption. }
+      * eapply Rename.term_det; try reflexivity; try eassumption.
+        eapply Map.bulk_overwrite_det; try eassumption. apply Map.eq_refl.
+      * eapply Rename.term_det; try reflexivity; try eassumption.
+        eapply Map.bulk_overwrite_det; try eassumption. apply Map.eq_refl.
+Qed.
