theories/WellFormed.v
@@ -1,0 +1,34 @@
+From LinearCore Require
+  BoundIn
+  Pattern
+  .
+
+
+
+Inductive Strict : Pattern.strict -> Prop :=
+  | SCtr constructor
+      : Strict (Pattern.Ctr constructor)
+  | SApp curried (curried_well_formed : Strict curried) argument (N : forall (B : BoundIn.Strict curried argument), False)
+      : Strict (Pattern.App curried argument)
+  .
+Arguments Strict strict.
+
+
+
+Inductive MoveOrReference : Pattern.move_or_reference -> Prop :=
+  | MMov strict (strict_well_formed : Strict strict)
+      : MoveOrReference (Pattern.Mov strict)
+  | MRef strict (strict_well_formed : Strict strict)
+      : MoveOrReference (Pattern.Ref strict)
+  .
+Arguments MoveOrReference move_or_reference.
+
+
+
+Inductive Pattern : Pattern.pattern -> Prop :=
+  | Nam name
+      : Pattern (Pattern.Nam name)
+  | Pat move_or_reference (move_or_reference_well_formed : MoveOrReference move_or_reference)
+      : Pattern (Pattern.Pat move_or_reference)
+  .
+Arguments Pattern pattern.
